initial changes

Weidenbach_Book/IsaSAT_Propagate_Conflict.thy
@@ -1,5 +1,5 @@
 theory IsaSAT_Propagate_Conflict
-  imports IsaSAT_Setup
+  imports IsaSAT_Setup Watched_Literals_Heuristics
 begin
 
 subsubsection \<open>Refining Propagate And Conflict\<close>
@@ -9,73 +9,12 @@ paragraph \<open>Propagation, Inner Loop\<close>
 context isasat_input_bounded
 begin
 
-lemma unit_prop_body_wl_invD:
-  fixes S w K
-  defines \<open>C \<equiv> (watched_by S K) ! w\<close>
-  assumes inv: \<open>unit_prop_body_wl_inv S w K\<close>
-  shows \<open>distinct((get_clauses_wl S)!C)\<close> and \<open>get_conflict_wl S = None\<close>
-proof -
-  obtain M N U D' NE UE Q W where
-     S: \<open>S = (M, N, U, D', NE, UE, Q, W)\<close>
-    by (cases S)
-  have
-     struct_invs: \<open>twl_struct_invs (twl_st_of (Some K) (st_l_of_wl (Some (K, w)) S))\<close> and
-     \<open>twl_list_invs (st_l_of_wl (Some (K, w)) S)\<close> and
-     corr: \<open>correct_watching S\<close> and
-     \<open>w < length (watched_by S K)\<close> and
-     confl: \<open>get_conflict_wl S = None\<close> and
-     w_ge_0: \<open>0 < watched_by S K ! w\<close> and
-     w_le_length: \<open>w < length (watched_by S K)\<close> and
-     w_le_length_S: \<open>watched_by S K ! w < length (get_clauses_wl S)\<close>
-    using inv unfolding unit_prop_body_wl_inv_def by fast+
-
-  show \<open>get_conflict_wl S = None\<close>
-    using confl .
-  have \<open>cdcl\<^sub>W_restart_mset.cdcl\<^sub>W_all_struct_inv
-       (state\<^sub>W_of (twl_st_of (Some K) (st_l_of_wl (Some (K, w)) S)))\<close> and
-      \<open>\<forall>D\<in>#learned_clss (state\<^sub>W_of (twl_st_of (Some K) (st_l_of_wl (Some (K, w)) S))).
-      \<not> tautology D\<close>
-      and
-    dist: \<open>cdcl\<^sub>W_restart_mset.distinct_cdcl\<^sub>W_state
-    (state\<^sub>W_of (twl_st_of (Some K) (st_l_of_wl (Some (K, w)) S)))\<close>
-    using struct_invs unfolding twl_struct_invs_def
-      cdcl\<^sub>W_restart_mset.cdcl\<^sub>W_all_struct_inv_def
-    by fast+
-  have \<open>distinct_mset_set (mset ` set (tl N))\<close>
-    apply (subst append_take_drop_id[of \<open>U\<close> \<open>tl N\<close>, symmetric])
-    apply (subst set_append)
-    apply (subst image_Un)
-    apply (subst distinct_mset_set_union)
-    using dist
-    by (auto simp: C_def S cdcl\<^sub>W_restart_mset.distinct_cdcl\<^sub>W_state_def
-        mset_take_mset_drop_mset drop_Suc)
-  moreover have NC: \<open>N!C \<in> set (tl N)\<close>
-     using w_ge_0 w_le_length_S unfolding C_def S
-     by (auto intro!: nth_in_set_tl)
-  ultimately show \<open>distinct((get_clauses_wl S)!C)\<close>
-     unfolding distinct_mset_set_def S by simp
-qed
-
 lemma (in -)[sepref_fr_rules]:
   \<open>(return o id, RETURN o nat_of_lit) \<in> unat_lit_assn\<^sup>k \<rightarrow>\<^sub>a uint32_nat_assn\<close>
   by sepref_to_hoare
      (sep_auto simp: uint32_nat_rel_def br_def unat_lit_rel_def nat_lit_rel_def
       lit_of_natP_def)
 
-fun watched_by_int:: \<open>twl_st_wl_heur \<Rightarrow> nat literal \<Rightarrow> watched\<close> where
-  \<open>watched_by_int (M, N, U, D, Q, W, _) L = W ! nat_of_lit L\<close>
-
-fun (in -) get_watched_wl :: \<open>nat twl_st_wl \<Rightarrow> (nat literal \<Rightarrow> nat list)\<close> where
-  \<open>get_watched_wl (_, _, _, _, _, _, _, W) = W\<close>
-
-fun (in -) get_watched_wl_heur :: \<open>twl_st_wl_heur \<Rightarrow> nat list list\<close> where
-  \<open>get_watched_wl_heur (_, _, _, _, _, W, _) = W\<close>
-
-definition (in -) watched_by_app_heur :: \<open>twl_st_wl_heur \<Rightarrow> nat literal \<Rightarrow> nat \<Rightarrow> nat\<close> where
-  \<open>watched_by_app_heur = (\<lambda>(M, N, U, D, Q, W, _) L K. W ! nat_of_lit L ! K)\<close>
-
-definition (in -) watched_by_app :: \<open>nat twl_st_wl \<Rightarrow> nat literal \<Rightarrow> nat \<Rightarrow> nat\<close> where
-  \<open>watched_by_app S L K = watched_by S L ! K\<close>
 
 lemma watched_by_app_watched_by_app_heur:
   \<open>(uncurry2 (RETURN ooo watched_by_app_heur), uncurry2 (RETURN ooo watched_by_app)) \<in>
@@ -86,11 +25,11 @@ lemma watched_by_app_watched_by_app_heur:
 
 sepref_thm watched_by_app_heur_code
   is \<open>uncurry2 (RETURN ooo watched_by_app_heur)\<close>
-  :: \<open>[\<lambda>((S, L), K). nat_of_lit L < length (get_watched_wl_heur S) \<and>
-          K < length (watched_by_int S L)]\<^sub>a
+  :: \<open>[watched_by_app_heur_pre]\<^sub>a
         twl_st_heur_assn\<^sup>k *\<^sub>a unat_lit_assn\<^sup>k *\<^sub>a nat_assn\<^sup>k \<rightarrow> nat_assn\<close>
   supply [[goals_limit=1]]
-  unfolding watched_by_app_heur_def twl_st_heur_assn_def nth_rll_def[symmetric]
+  unfolding watched_by_app_heur_alt_def twl_st_heur_assn_def nth_rll_def[symmetric]
+   watched_by_app_heur_pre_def
   by sepref
 
 concrete_definition (in -) watched_by_app_heur_code
@@ -102,6 +41,7 @@ prepare_code_thms (in -) watched_by_app_heur_code_def
 lemmas watched_by_app_heur_code_refine[sepref_fr_rules] =
    watched_by_app_heur_code.refine[of \<A>\<^sub>i\<^sub>n, OF isasat_input_bounded_axioms]
 
+(* TODO Kill *)
 lemma watched_by_app_code_refine[sepref_fr_rules]:
   \<open>(uncurry2 watched_by_app_heur_code, uncurry2 (RETURN ooo watched_by_app)) \<in>
     [\<lambda>((S, L), K).  L \<in> snd ` D\<^sub>0 \<and> K < length (watched_by S L)]\<^sub>a
@@ -120,7 +60,8 @@ proof -
     hr_comp nat_assn nat_rel\<close>
     (is \<open>_ \<in> [?pre']\<^sub>a ?im' \<rightarrow> ?f'\<close>)
     using hfref_compI_PRE_aux[OF watched_by_app_heur_code_refine[unfolded PR_CONST_def]
-        watched_by_app_watched_by_app_heur[unfolded PR_CONST_def]] .
+        watched_by_app_watched_by_app_heur[unfolded PR_CONST_def],
+        unfolded watched_by_app_heur_pre_def] .
   have pre: \<open>?pre' = ?pre\<close>
     by (intro ext) (auto simp: comp_PRE_def twl_st_assn_def twl_st_heur_def map_fun_rel_def)
   have im: \<open>?im' = ?im\<close>
@@ -134,110 +75,13 @@ proof -
 qed
 
 
-lemma unit_prop_body_wl_D_invD:
-  assumes \<open>unit_prop_body_wl_D_inv S w L\<close>
-  shows
-    \<open>w < length (watched_by S L)\<close> and
-    \<open>watched_by_app S L w < length (get_clauses_wl S)\<close> and
-    \<open>get_clauses_wl S ! watched_by_app S L w \<noteq> []\<close> and
-    \<open>Suc 0 < length (get_clauses_wl S ! watched_by_app S L w)\<close> and
-    \<open>get_clauses_wl S ! watched_by_app S L w ! 0 \<in> snd ` D\<^sub>0\<close> and
-    \<open>get_clauses_wl S ! watched_by_app S L w ! Suc 0 \<in> snd ` D\<^sub>0\<close> and
-    \<open>L \<in> snd ` D\<^sub>0\<close> and
-    \<open>watched_by_app S L w > 0\<close> and
-    \<open>literals_are_\<L>\<^sub>i\<^sub>n S\<close> and
-    \<open>get_conflict_wl S = None\<close> and
-    \<open>literals_are_in_\<L>\<^sub>i\<^sub>n (mset (get_clauses_wl S ! watched_by_app S L w))\<close> and
-    \<open>distinct (get_clauses_wl S ! watched_by_app S L w)\<close>
-proof -
-  show \<open>L \<in> snd ` D\<^sub>0\<close>
-    using assms unfolding unit_prop_body_wl_D_inv_def by fast
-  show \<open>w < length (watched_by S L)\<close>
-    using assms unfolding unit_prop_body_wl_D_inv_def unit_prop_body_wl_inv_def by fast
-  show S_L_W_le_S: \<open>watched_by_app S L w < length (get_clauses_wl S)\<close>
-    using assms unfolding unit_prop_body_wl_D_inv_def unit_prop_body_wl_inv_def watched_by_app_def
-    by fast
-  show \<open>get_clauses_wl S ! watched_by_app S L w \<noteq> []\<close>
-    using assms twl_struct_invs_length_clause_ge_2[of L w S \<open>watched_by S L ! w\<close>]
-    unfolding unit_prop_body_wl_D_inv_def unit_prop_body_wl_inv_def watched_by_app_def
-      twl_list_invs_def by force
-  show le: \<open>Suc 0 < length (get_clauses_wl S ! watched_by_app S L w)\<close>
-    using assms twl_struct_invs_length_clause_ge_2[of L w S \<open>watched_by S L ! w\<close>]
-    unfolding unit_prop_body_wl_D_inv_def unit_prop_body_wl_inv_def watched_by_app_def
-      twl_list_invs_def by force
-  have nempty: \<open>get_clauses_wl S \<noteq> []\<close> and S_L_w_ge_0: \<open>0 < watched_by_app S L w\<close>
-    using assms unfolding unit_prop_body_wl_D_inv_def unit_prop_body_wl_inv_def
-    twl_list_invs_def watched_by_app_def by auto
-  obtain M N U D NE UE W Q where
-    S: \<open>S = (M, N, U, D, NE, UE, Q, W)\<close>
-    by (cases S)
-  show lits_N: \<open>literals_are_in_\<L>\<^sub>i\<^sub>n (mset (get_clauses_wl S ! watched_by_app S L w))\<close>
-    using assms unfolding unit_prop_body_wl_D_inv_def apply -
-    apply (rule literals_are_in_\<L>\<^sub>i\<^sub>n_nth[of _ _ M U D NE UE Q W])
-    apply (rule S_L_W_le_S)
-    apply (rule S_L_w_ge_0)
-    using S by (auto simp del: twl_st_of.simps)
-  then show \<open>get_clauses_wl S ! watched_by_app S L w ! 0 \<in> snd ` D\<^sub>0\<close>
-    using le apply (cases \<open>get_clauses_wl S ! watched_by_app S L w\<close>;
-        cases \<open>tl (get_clauses_wl S ! watched_by_app S L w)\<close>)
-    by (auto simp: literals_are_in_\<L>\<^sub>i\<^sub>n_def all_lits_of_m_add_mset)
-
-  show \<open>get_clauses_wl S ! watched_by_app S L w ! Suc 0 \<in> snd ` D\<^sub>0\<close>
-    using lits_N le apply (cases \<open>get_clauses_wl S ! watched_by_app S L w\<close>;
-        cases \<open>tl (get_clauses_wl S ! watched_by_app S L w)\<close>;
-        cases \<open>tl (tl (get_clauses_wl S ! watched_by_app S L w))\<close>)
-    by (auto simp: literals_are_in_\<L>\<^sub>i\<^sub>n_def all_lits_of_m_add_mset)
-
-  show S_L_W_ge_0: \<open>watched_by_app S L w > 0\<close> and
-    \<open>literals_are_\<L>\<^sub>i\<^sub>n S\<close> and
-    \<open>get_conflict_wl S = None\<close>
-    using assms unfolding unit_prop_body_wl_D_inv_def unit_prop_body_wl_inv_def watched_by_app_def
-    by fast+
-  have
-    struct: \<open>twl_struct_invs (twl_st_of (Some L) (st_l_of_wl (Some (L, w)) S))\<close> and
-    stgy: \<open>twl_stgy_invs (twl_st_of (Some L) (st_l_of_wl (Some (L, w)) S))\<close>
-    using assms unfolding unit_prop_body_wl_D_inv_def unit_prop_body_wl_inv_def watched_by_app_def
-    by fast+
-  have
-    all_inv: \<open>cdcl\<^sub>W_restart_mset.cdcl\<^sub>W_all_struct_inv
-          (state\<^sub>W_of (twl_st_of (Some L) (st_l_of_wl (Some (L, w)) S)))\<close>
-    using struct unfolding twl_struct_invs_def by fast+
-  then have
-     learned_tauto:
-       \<open>\<forall>s\<in>#learned_clss (state\<^sub>W_of (twl_st_of (Some L) (st_l_of_wl (Some (L, w)) S))).
-           \<not> tautology s\<close> and
-     dist:
-        \<open>cdcl\<^sub>W_restart_mset.distinct_cdcl\<^sub>W_state (state\<^sub>W_of (twl_st_of (Some L)
-            (st_l_of_wl (Some (L, w)) S)))\<close>
-    using struct unfolding cdcl\<^sub>W_restart_mset.cdcl\<^sub>W_all_struct_inv_def by fast+
-  have \<open>\<forall>D\<in>mset ` set (tl (get_clauses_wl S)). distinct_mset D\<close>
-    apply (subst append_take_drop_id[of \<open>get_learned_wl S\<close>, symmetric])
-    unfolding set_append
-    using dist
-    apply (cases S)
-    by (auto simp: drop_Suc clauses_def mset_take_mset_drop_mset
-        watched_by_app_def cdcl\<^sub>W_restart_mset.distinct_cdcl\<^sub>W_state_def distinct_mset_set_distinct)
-  then show \<open>distinct (get_clauses_wl S ! watched_by_app S L w)\<close>
-    using S_L_W_le_S S_L_W_ge_0 nempty
-    by (cases S; cases \<open>get_clauses_wl S\<close>)
-       (auto simp: cdcl\<^sub>W_restart_mset.distinct_cdcl\<^sub>W_state_def distinct_mset_set_distinct
-         clauses_def mset_take_mset_drop_mset watched_by_app_def)
-qed
-
-definition (in -) access_lit_in_clauses where
-  \<open>access_lit_in_clauses S i j = (get_clauses_wl S) ! i ! j\<close>
-
-definition (in -) access_lit_in_clauses_heur where
-  \<open>access_lit_in_clauses_heur = (\<lambda>(M, N, _) i j.  N ! i ! j)\<close>
-
-
 sepref_thm access_lit_in_clauses_heur_code
   is \<open>uncurry2 (RETURN ooo access_lit_in_clauses_heur)\<close>
-  :: \<open>[\<lambda>(((_,N,_), i), j). i < length N \<and> j < length_rll N i]\<^sub>a
+  :: \<open>[access_lit_in_clauses_heur_pre]\<^sub>a
       twl_st_heur_assn\<^sup>k *\<^sub>a nat_assn\<^sup>k  *\<^sub>a nat_assn\<^sup>k \<rightarrow> unat_lit_assn\<close>
   supply length_rll_def[simp]
-  unfolding twl_st_heur_assn_def access_lit_in_clauses_heur_def
-    nth_rll_def[symmetric]
+  unfolding twl_st_heur_assn_def access_lit_in_clauses_heur_alt_def
+    nth_rll_def[symmetric] access_lit_in_clauses_heur_pre_def
   by sepref
 
 concrete_definition (in -) access_lit_in_clauses_heur_code
@@ -256,6 +100,7 @@ lemma access_lit_in_clauses_heur_access_lit_in_clauses:
   by (intro frefI nres_relI)
      (auto simp: access_lit_in_clauses_heur_def twl_st_heur_def access_lit_in_clauses_def)
 
+(* TODO Kill *)
 lemma access_lit_in_clauses_refine[sepref_fr_rules]:
   \<open>(uncurry2 access_lit_in_clauses_heur_code, uncurry2 (RETURN ooo access_lit_in_clauses)) \<in>
     [\<lambda>((S, i), j). i < length (get_clauses_wl S) \<and> j < length_rll (get_clauses_wl S) i]\<^sub>a
@@ -271,7 +116,8 @@ proof -
     hr_comp unat_lit_assn Id\<close>
     (is \<open>_ \<in> [?pre']\<^sub>a ?im' \<rightarrow> ?f'\<close>)
     using hfref_compI_PRE_aux[OF access_lit_in_clauses_heur_code_refine[unfolded PR_CONST_def]
-        access_lit_in_clauses_heur_access_lit_in_clauses[unfolded PR_CONST_def]] .
+        access_lit_in_clauses_heur_access_lit_in_clauses[unfolded PR_CONST_def],
+        unfolded access_lit_in_clauses_heur_pre_def] .
   have pre: \<open>?pre x \<Longrightarrow> ?pre' x\<close> for x
     unfolding comp_PRE_def
       by (auto simp: comp_PRE_def twl_st_assn_def twl_st_heur_def
@@ -288,38 +134,6 @@ proof -
     using H unfolding im f apply assumption
     using pre ..
 qed
-
-definition (in -) find_unwatched_wl_st  :: \<open>nat twl_st_wl \<Rightarrow> nat \<Rightarrow> nat option nres\<close> where
-\<open>find_unwatched_wl_st = (\<lambda>(M, N, U, D, NE, UE, Q, W) i. do {
-    find_unwatched_l M (N ! i)
-  })\<close>
-
-lemma find_unwatched_l_find_unwatched_wl_s:
-  \<open>find_unwatched_l (get_trail_wl S) (get_clauses_wl S ! C) = find_unwatched_wl_st S C\<close>
-  by (cases S) (auto simp: find_unwatched_wl_st_def)
-
-definition (in -) find_unwatched :: \<open>('a, 'b) ann_lits \<Rightarrow> 'a clause_l \<Rightarrow> (nat option) nres\<close> where
-\<open>find_unwatched M C = do {
-   S \<leftarrow> WHILE\<^sub>T\<^bsup>\<lambda>(found, i). i \<ge> 2 \<and> i \<le> length C \<and> (\<forall>j\<in>{2..<i}. -(C!j) \<in> lits_of_l M) \<and>
-      (\<forall>j. found = Some j \<longrightarrow> (i = j \<and> (undefined_lit M (C!j) \<or> C!j \<in> lits_of_l M) \<and>
-       j < length C \<and> j \<ge> 2))\<^esup>
-    (\<lambda>(found, i). found = None \<and> i < length C)
-    (\<lambda>(_, i). do {
-      ASSERT(i < length C);
-      case polarity M (C!i) of
-        None \<Rightarrow> do { RETURN (Some i, i)}
-      | Some v \<Rightarrow>
-         (if v then do { RETURN (Some i, i)} else do { RETURN (None, i+1)})
-    })
-    (None, 2::nat);
-  RETURN (fst S)
-  }
-\<close>
-
-definition find_unwatched_wl_st_heur  :: \<open>twl_st_wl_heur \<Rightarrow> nat \<Rightarrow> nat option nres\<close> where
-\<open>find_unwatched_wl_st_heur = (\<lambda>(M, N, U, D, Q, W, vm, \<phi>) i. do {
-    find_unwatched M (N ! i)
-  })\<close>
 
 end
 
@@ -338,13 +152,13 @@ begin
 
 sepref_thm find_unwatched_wl_st_heur_code
   is \<open>uncurry ((PR_CONST find_unwatched_wl_st_heur))\<close>
-  :: \<open>[\<lambda>(S, i). i < length (get_clauses_wl_heur S) \<and> i > 0 \<and> literals_are_in_\<L>\<^sub>i\<^sub>n_heur S]\<^sub>a
+  :: \<open>[find_unwatched_wl_st_heur_pre]\<^sub>a
          twl_st_heur_assn\<^sup>k *\<^sub>a nat_assn\<^sup>k \<rightarrow> option_assn nat_assn\<close>
   supply [[goals_limit = 1]] literals_are_in_\<L>\<^sub>i\<^sub>n_heur_in_D\<^sub>0'[intro] nth_rll_def[simp]
     length_rll_def[simp]
   unfolding find_unwatched_wl_st_heur_def twl_st_heur_assn_def PR_CONST_def
   find_unwatched_def nth_rll_def[symmetric] length_rll_def[symmetric]
-  case_tri_bool_If
+  case_tri_bool_If find_unwatched_wl_st_heur_pre_def
   by sepref
 
 concrete_definition (in -) find_unwatched_wl_st_heur_code
@@ -354,74 +168,10 @@ concrete_definition (in -) find_unwatched_wl_st_heur_code
 prepare_code_thms (in -) find_unwatched_wl_st_heur_code_def
 
 lemmas find_unwatched_wl_st_heur_code_find_unwatched_wl_st_heur[sepref_fr_rules] =
-   find_unwatched_wl_st_heur_code.refine[of \<A>\<^sub>i\<^sub>n, OF isasat_input_bounded_nempty_axioms]
+   find_unwatched_wl_st_heur_code.refine[of \<A>\<^sub>i\<^sub>n, OF isasat_input_bounded_nempty_axioms,
+     unfolded PR_CONST_def]
 
-lemma (in -) find_unwatched:
-  assumes \<open>no_dup M\<close> and \<open>length C \<ge> 2\<close>
-  shows \<open>find_unwatched M C \<le> find_unwatched_l M C\<close>
-  unfolding find_unwatched_def find_unwatched_l_def
-  apply (refine_vcg WHILEIT_rule[where R = \<open>measure (\<lambda>(found, i). Suc (length C) - i +
-        If (found = None) 1 0)\<close>])
-  subgoal by auto
-  subgoal by auto
-  subgoal using assms by auto
-  subgoal by auto
-  subgoal by auto
-  subgoal by auto
-  subgoal by auto
-  subgoal by auto
-  subgoal by auto
-  subgoal by auto
-  subgoal for s
-    by (auto simp: Decided_Propagated_in_iff_in_lits_of_l not_less_less_Suc_eq polarity_def
-        split: if_splits intro!: exI[of _ \<open>snd s - 2\<close>])
-  subgoal for s
-    by (auto simp: Decided_Propagated_in_iff_in_lits_of_l not_less_less_Suc_eq
-        split: if_splits intro: exI[of _ \<open>snd s - 2\<close>])
-  subgoal for s
-    by (auto simp: Decided_Propagated_in_iff_in_lits_of_l not_less_less_Suc_eq polarity_def
-        split: if_splits intro: exI[of _ \<open>snd s - 2\<close>])
-  subgoal by (auto simp: polarity_def split: if_splits)
-  subgoal by auto
-  subgoal by auto
-  subgoal by auto
-  subgoal by auto
-  subgoal by auto
-  subgoal by auto
-  subgoal by auto
-  subgoal by (auto simp: polarity_def split: if_splits)
-  subgoal by auto
-  subgoal by auto
-  subgoal by auto
-  subgoal by auto
-  subgoal by auto
-  subgoal for s using distinct_consistent_interp[OF assms(1)]
-    apply (auto simp: Decided_Propagated_in_iff_in_lits_of_l consistent_interp_def all_set_conv_nth
-       polarity_def split: if_splits intro: exI[of _ \<open>snd s - 2\<close>])
-    by (metis atLeastLessThan_iff less_antisym)
-  subgoal by auto
-  subgoal by auto
-  subgoal by auto
-  subgoal by auto
-  subgoal by auto
-  subgoal for s using no_dup_consistentD[OF assms(1)]
-    by (cases s, cases \<open>fst s\<close>)
-      (auto simp: Decided_Propagated_in_iff_in_lits_of_l all_set_conv_nth
-        intro!: exI[of _ \<open>snd s - 2\<close>])
-  subgoal by auto
-  subgoal for s j by auto
-  subgoal by auto
-  done
-
-theorem find_unwatched_wl_st_heur_find_unwatched_wl_s:
-  \<open>(uncurry find_unwatched_wl_st_heur, uncurry find_unwatched_wl_st)
-    \<in> [\<lambda>(S, i). i < length (get_clauses_wl S) \<and> 0 < i \<and> literals_are_\<L>\<^sub>i\<^sub>n S \<and>
-      length (get_clauses_wl S ! i) \<ge> 2]\<^sub>f
-      twl_st_heur \<times>\<^sub>f nat_rel \<rightarrow> \<langle>Id\<rangle>nres_rel\<close>
-  by (intro frefI nres_relI)
-     (auto simp: find_unwatched_wl_st_def find_unwatched_wl_st_heur_def twl_st_heur_def
-    find_unwatched)
-
+(* TODO Kill *)
 theorem find_unwatched_wl_st_heur_code_find_unwatched_wl_s[sepref_fr_rules]:
   \<open>(uncurry find_unwatched_wl_st_heur_code, uncurry find_unwatched_wl_st)
     \<in> [\<lambda>(S, i). \<exists>w L. unit_prop_body_wl_D_inv S w L \<and> i = watched_by_app S L w]\<^sub>a
@@ -440,7 +190,8 @@ proof -
     (is \<open>_ \<in> [?pre']\<^sub>a ?im' \<rightarrow> ?f'\<close>)
     using hfref_compI_PRE_aux[OF
         find_unwatched_wl_st_heur_code_find_unwatched_wl_st_heur[unfolded PR_CONST_def]
-        find_unwatched_wl_st_heur_find_unwatched_wl_s] .
+        find_unwatched_wl_st_heur_find_unwatched_wl_s,
+         unfolded find_unwatched_wl_st_heur_pre_def] .
   have pre: \<open>?pre' x\<close> if \<open>?pre x\<close> for x
   proof -
     have [simp]: \<open>mset `# mset (take ai (tl ah)) + ak + (mset `# mset (drop (Suc ai) ah) + al) =
@@ -485,59 +236,27 @@ proof -
     using pre ..
 qed
 
-lemmas unit_prop_body_wl_D_invD' =
-  unit_prop_body_wl_D_invD[of \<open>(M, N, U, D, NE, UE, WS, Q)\<close> for M N U D NE UE WS Q,
-   unfolded watched_by_app_def,
-    simplified] unit_prop_body_wl_D_invD(7)
 
-definition set_conflict_wl' :: \<open>nat \<Rightarrow> 'v twl_st_wl \<Rightarrow> 'v twl_st_wl\<close> where
-  \<open>set_conflict_wl' = (\<lambda>C (M, N, U, D, NE, UE, Q, W). (M, N, U, Some (mset (N!C)), NE, UE, {#}, W))\<close>
-
-lemma set_conflict_wl'_alt_def:
-  \<open>set_conflict_wl' i S = set_conflict_wl (get_clauses_wl S ! i) S\<close>
-  by (cases S) (auto simp: set_conflict_wl'_def set_conflict_wl_def)
-
-definition set_conflict_wl'_int :: \<open>nat \<Rightarrow> twl_st_wl_heur \<Rightarrow> twl_st_wl_heur nres\<close> where
-  \<open>set_conflict_wl'_int = (\<lambda>C (M, N, U, D, Q, W, vmtf, \<phi>, clvls, cach, lbd, stats). do {
-    let n = zero_uint32_nat;
-    (D, clvls, lbd) \<leftarrow> set_conflict_m M N C D n lbd;
-    RETURN (M, N, U, D, {#}, W, vmtf, \<phi>, clvls, cach, lbd, incr_conflict stats)})\<close>
-
-sepref_thm set_conflict_wl'_int_code
-  is \<open>uncurry set_conflict_wl'_int\<close>
-  :: \<open>[\<lambda>(C, S). get_conflict_wl_heur S = None \<and> C < length (get_clauses_wl_heur S) \<and>
-        distinct (get_clauses_wl_heur S ! C) \<and>
-        literals_are_in_\<L>\<^sub>i\<^sub>n (mset (get_clauses_wl_heur S ! C)) \<and>
-        \<not> tautology (mset (get_clauses_wl_heur S ! C)) \<and>
-        literals_are_in_\<L>\<^sub>i\<^sub>n_trail (get_trail_wl_heur S) \<and>
-        no_dup (get_trail_wl_heur S)]\<^sub>a
+sepref_thm set_conflict_wl_heur_code
+  is \<open>uncurry set_conflict_wl_heur\<close>
+  :: \<open>[set_conflict_wl_heur_pre]\<^sub>a
     nat_assn\<^sup>k *\<^sub>a twl_st_heur_assn\<^sup>d \<rightarrow> twl_st_heur_assn\<close>
   supply [[goals_limit=1]]
-  unfolding set_conflict_wl'_int_def twl_st_heur_assn_def IICF_List_Mset.lms_fold_custom_empty
+  unfolding set_conflict_wl_heur_def twl_st_heur_assn_def IICF_List_Mset.lms_fold_custom_empty
+    set_conflict_wl_heur_pre_def
   by sepref
 
-concrete_definition (in -) set_conflict_wl'_int_code
-  uses isasat_input_bounded_nempty.set_conflict_wl'_int_code.refine_raw
+concrete_definition (in -) set_conflict_wl_heur_code
+  uses isasat_input_bounded_nempty.set_conflict_wl_heur_code.refine_raw
   is \<open>(uncurry ?f, _)\<in>_\<close>
 
-prepare_code_thms (in -) set_conflict_wl'_int_code_def
+prepare_code_thms (in -) set_conflict_wl_heur_code_def
 
-lemmas set_conflict_wl'_int_code[sepref_fr_rules] =
-  set_conflict_wl'_int_code.refine[OF isasat_input_bounded_nempty_axioms]
+lemmas set_conflict_wl_heur_code[sepref_fr_rules] =
+  set_conflict_wl_heur_code.refine[OF isasat_input_bounded_nempty_axioms]
 
-
-lemma set_conflict_wl'_int_set_conflict_wl':
-  \<open>(uncurry set_conflict_wl'_int, uncurry (RETURN oo set_conflict_wl')) \<in>
-    nat_rel \<times>\<^sub>r twl_st_heur \<rightarrow>\<^sub>f \<langle>twl_st_heur\<rangle>nres_rel\<close>
-  by (intro nres_relI frefI)
-    (auto simp: twl_st_heur_def set_conflict_wl'_int_def set_conflict_wl'_def
-        bind_RES_RETURN2_eq RETURN_def RES_RES2_RETURN_RES
-        counts_maximum_level_def RES_RETURN_RES3 RES_RES_RETURN_RES RES_RES3_RETURN_RES
-        set_conflict_m_def
-      intro!: RES_refine)
-
-lemma set_conflict_wl'_int_code_set_conflict_wl'[sepref_fr_rules]:
-  \<open>(uncurry set_conflict_wl'_int_code, uncurry (RETURN oo set_conflict_wl')) \<in>
+lemma set_conflict_wl_heur_code_set_conflict_wl'[sepref_fr_rules]:
+  \<open>(uncurry set_conflict_wl_heur_code, uncurry (RETURN oo set_conflict_wl')) \<in>
     [\<lambda>(C, S). get_conflict_wl S = None \<and> C < length (get_clauses_wl S) \<and>
       distinct (get_clauses_wl S ! C) \<and> literals_are_in_\<L>\<^sub>i\<^sub>n (mset (get_clauses_wl S ! C)) \<and>
       \<not> tautology (mset (get_clauses_wl S ! C)) \<and>
@@ -545,28 +264,19 @@ lemma set_conflict_wl'_int_code_set_conflict_wl'[sepref_fr_rules]:
     twl_st_assn\<close>
     (is \<open>_ \<in> [?pre]\<^sub>a ?im \<rightarrow> ?f\<close>)
 proof -
-  have H: \<open>(uncurry set_conflict_wl'_int_code, uncurry (RETURN \<circ>\<circ> set_conflict_wl'))
+  have H: \<open>(uncurry set_conflict_wl_heur_code, uncurry (RETURN \<circ>\<circ> set_conflict_wl'))
   \<in> [comp_PRE (nat_rel \<times>\<^sub>f twl_st_heur) (\<lambda>_. True)
-       (\<lambda>_ (C, S).
-           get_conflict_wl_heur S = None \<and>
-           C < length (get_clauses_wl_heur S) \<and>
-           distinct (get_clauses_wl_heur S ! C) \<and>
-           literals_are_in_\<L>\<^sub>i\<^sub>n
-            (mset (get_clauses_wl_heur S ! C)) \<and>
-           \<not> tautology (mset (get_clauses_wl_heur S ! C)) \<and>
-           literals_are_in_\<L>\<^sub>i\<^sub>n_trail
-            (get_trail_wl_heur S) \<and>
-           no_dup (get_trail_wl_heur S))
+       (\<lambda>_. set_conflict_wl_heur_pre)
        (\<lambda>_. True)]\<^sub>a hrp_comp
                        (nat_assn\<^sup>k *\<^sub>a twl_st_heur_assn\<^sup>d)
                        (nat_rel \<times>\<^sub>f
                         twl_st_heur) \<rightarrow> hr_comp
            twl_st_heur_assn twl_st_heur\<close>
     (is \<open>_ \<in> [?pre']\<^sub>a ?im' \<rightarrow> ?f'\<close>)
-    using hfref_compI_PRE_aux[OF set_conflict_wl'_int_code set_conflict_wl'_int_set_conflict_wl']
+    using hfref_compI_PRE_aux[OF set_conflict_wl_heur_code set_conflict_wl_heur_set_conflict_wl']
     .
   have pre: \<open>?pre' x\<close> if \<open>?pre x\<close> for x
-    using that unfolding comp_PRE_def twl_st_heur_def by auto
+    using that unfolding comp_PRE_def twl_st_heur_def set_conflict_wl_heur_pre_def by auto
   have im: \<open>?im' = ?im\<close>
     unfolding prod_hrp_comp hrp_comp_dest hrp_comp_keep twl_st_assn_def[symmetric]
     by (auto simp: hrp_comp_def hr_comp_def)
@@ -580,47 +290,17 @@ proof -
     using pre ..
 qed
 
-
-definition update_clause_wl_heur :: \<open>nat literal \<Rightarrow> nat \<Rightarrow> nat \<Rightarrow> nat \<Rightarrow> nat \<Rightarrow> twl_st_wl_heur \<Rightarrow>
-    (nat \<times> twl_st_wl_heur) nres\<close> where
-  \<open>update_clause_wl_heur = (\<lambda>(L::nat literal) C w i f (M, N, U, D, Q, W, vm). do {
-     let K' = (N!C) ! f;
-     let N' = list_update N C (swap (N!C) i f);
-     let W = W[nat_of_lit L := delete_index_and_swap (W ! nat_of_lit L) w];
-     RETURN (w, (M, N', U, D, Q,
-            W[nat_of_lit K':= W ! nat_of_lit K' @ [C]],
-            vm))
-  })\<close>
-
-lemma update_clause_wl_heur_update_clause_wl:
-  \<open>(uncurry5 update_clause_wl_heur, uncurry5 (update_clause_wl)) \<in>
-   [\<lambda>(((((L, C), w), i), f), S). (get_clauses_wl S ! C) ! f \<noteq> L]\<^sub>f
-   Id \<times>\<^sub>f nat_rel \<times>\<^sub>f nat_rel \<times>\<^sub>f nat_rel \<times>\<^sub>f nat_rel \<times>\<^sub>f twl_st_heur \<rightarrow>
-  \<langle>nat_rel \<times>\<^sub>r twl_st_heur\<rangle>nres_rel\<close>
-  by (intro frefI nres_relI)
-    (auto simp: update_clause_wl_heur_def update_clause_wl_def twl_st_heur_def Let_def
-      map_fun_rel_def)
-
-lemma length_delete_index_and_swap_ll[simp]: \<open>length (delete_index_and_swap_ll s i j) = length s\<close>
-  by (auto simp: delete_index_and_swap_ll_def)
-
 sepref_thm update_clause_wl_code
   is \<open>uncurry5 update_clause_wl_heur\<close>
   :: \<open>
-    [\<lambda>(((((L, C), w), i), f), S).
-      C < length (get_clauses_wl_heur S) \<and>
-      f < length (get_clauses_wl_heur S ! C) \<and>
-      i < length (get_clauses_wl_heur S ! C) \<and>
-      nat_of_lit L < length (get_watched_wl_heur S) \<and>
-      nat_of_lit ((get_clauses_wl_heur S ! C) ! f)  < length (get_watched_wl_heur S) \<and>
-      w < length (get_watched_wl_heur S ! nat_of_lit L)]\<^sub>a
+    [update_clause_wl_code_pre]\<^sub>a
      unat_lit_assn\<^sup>k *\<^sub>a nat_assn\<^sup>k *\<^sub>a nat_assn\<^sup>k *\<^sub>a nat_assn\<^sup>k *\<^sub>a nat_assn\<^sup>k *\<^sub>a twl_st_heur_assn\<^sup>d \<rightarrow>
        nat_assn *a twl_st_heur_assn\<close>
   supply [[goals_limit=1]] length_rll_def[simp] length_ll_def[simp]
   unfolding update_clause_wl_heur_def twl_st_heur_assn_def Array_List_Array.swap_ll_def[symmetric]
     nth_rll_def[symmetric] delete_index_and_swap_update_def[symmetric]
     delete_index_and_swap_ll_def[symmetric]
-    append_ll_def[symmetric]
+    append_ll_def[symmetric] update_clause_wl_code_pre_def
   by sepref
 
 
@@ -633,155 +313,7 @@ prepare_code_thms (in -) update_clause_wl_code_def
 lemmas update_clause_wl_code[sepref_fr_rules] =
   update_clause_wl_code.refine[OF isasat_input_bounded_nempty_axioms]
 
-lemma
-  find_unwatched_not_tauto:
-    \<open>\<not>tautology(mset (get_clauses_wl S ! watched_by_app S L C))\<close>
-    (is ?tauto is \<open>\<not>tautology (?D)\<close> is \<open>\<not>tautology (mset ?C)\<close>)
-  if
-    find_unw: \<open>unit_prop_body_wl_D_find_unwatched_inv None (watched_by_app S L C) S\<close> and
-    inv: \<open>unit_prop_body_wl_D_inv S C L\<close> and
-    val: \<open>polarity_st S (get_clauses_wl S ! watched_by_app S L C !
-         (1 - (if access_lit_in_clauses S (watched_by_app S L C) 0 = L then 0 else 1))) =
-          Some False\<close>
-      (is \<open>polarity_st _ (_ ! _ ! ?i) = Some False\<close>)
-  for S C xj L
-proof  -
-  obtain M N U D NE UE WS Q where
-    S: \<open>S = (M, N, U, D, NE, UE, WS, Q)\<close>
-    by (cases S)
-
-  have \<open>consistent_interp
-       (lits_of_l (trail (state\<^sub>W_of (twl_st_of (Some L) (st_l_of_wl (Some (L, C)) S)))))\<close>
-    \<open>no_dup (trail (state\<^sub>W_of (twl_st_of (Some L) (st_l_of_wl (Some (L, C)) S))))\<close> and
-    valid: \<open>valid_enqueued (twl_st_of (Some L) (st_l_of_wl (Some (L, C)) S))\<close>
-    using inv unfolding unit_prop_body_wl_D_inv_def unit_prop_body_wl_inv_def twl_struct_invs_def
-      cdcl\<^sub>W_restart_mset.cdcl\<^sub>W_all_struct_inv_def cdcl\<^sub>W_restart_mset.cdcl\<^sub>W_M_level_inv_def
-    by blast+
-  then have cons: \<open>consistent_interp (lits_of_l (get_trail_wl S))\<close>
-    by (cases S) (auto)
-
-  have
-    \<open>twl_list_invs (st_l_of_wl (Some (L, C)) S)\<close> and
-    C_le: \<open>C < length (watched_by S L)\<close> and
-    confl: \<open>get_conflict_wl S = None\<close> and
-    \<open>no_duplicate_queued (twl_st_of (Some L) (st_l_of_wl (Some (L, C)) S))\<close>
-      using inv unfolding unit_prop_body_wl_D_inv_def unit_prop_body_wl_inv_def
-        unit_propagation_inner_loop_body_l_inv_def twl_struct_invs_def by fast+
-  have \<open>\<forall>L\<in>#mset (unwatched_l (get_clauses_wl S ! (watched_by S L ! C))).
-         - L \<in> lits_of_l (get_trail_wl S)\<close>
-    using find_unw unfolding unit_prop_body_wl_D_find_unwatched_inv_def
-      unit_prop_body_wl_find_unwatched_inv_def watched_by_app_def
-    by auto
-  moreover {
-    have
-      \<open>twl_list_invs (st_l_of_wl (Some (L, C)) S)\<close> and
-      \<open>C < length (watched_by S L)\<close> and
-      \<open>get_conflict_wl S = None\<close> and
-      \<open>no_duplicate_queued (twl_st_of (Some L) (st_l_of_wl (Some (L, C)) S))\<close>
-      using inv unfolding unit_prop_body_wl_D_inv_def unit_prop_body_wl_inv_def
-        unit_propagation_inner_loop_body_l_inv_def twl_struct_invs_def by fast+
-    then have \<open>add_mset L WS \<subseteq># {#- lit_of x. x \<in># mset (convert_lits_l N M)#}\<close>
-      apply (cases \<open>drop C (watched_by S L)\<close>)
-      apply (simp add: S image_image split: if_splits)
-      apply (simp add: S image_image split: if_splits)
-      unfolding ex_disj_distrib
-      by blast
-    from mset_subset_eq_insertD[OF this] have \<open>- L \<in> lits_of_l (convert_lits_l N M)\<close>
-      by (auto simp: lits_of_def)
-  }
-  moreover have \<open>- ?C ! ?i \<in> lits_of_l (convert_lits_l N M)\<close>
-    using val by (auto simp: S polarity_st_def watched_by_app_def polarity_def
-        access_lit_in_clauses_def Decided_Propagated_in_iff_in_lits_of_l split: if_splits)
-  moreover have length_C: \<open>length ?C \<ge> 2\<close>
-    apply (rule twl_struct_invs_length_clause_ge_2)
-    using inv unfolding unit_prop_body_wl_D_inv_def unit_prop_body_wl_inv_def
-    by (auto simp: watched_by_app_def)
-  moreover {
-    have QL: \<open>Q L ! C = hd (drop C (Q L))\<close>
-      using confl C_le length_C by (auto simp: S hd_drop_conv_nth split: )
-    have \<open>L \<in># mset (watched_l ?C)\<close>
-      using valid confl C_le length_C by (auto simp: QL S take_2_if watched_by_app_def)
-    then have \<open>N ! (Q L ! C) ! 0 = L \<or> N ! (Q L ! C) ! 1 = L\<close>
-      using confl C_le length_C by (auto simp: S take_2_if watched_by_app_def QL split: if_splits)
-  }
-  ultimately have Not: \<open>lits_of_l (get_trail_wl S) \<Turnstile>s CNot ?D\<close>
-    unfolding true_clss_def_iff_negation_in_model
-    apply (subst (2) append_take_drop_id[symmetric, of _ 2])
-    unfolding mset_append watched_by_app_def access_lit_in_clauses_def
-    by (auto simp: S take_2_if hd_conv_nth split: if_splits)
-  show ?thesis
-    using consistent_CNot_not_tautology[OF cons Not] .
-qed
-
-lemma
-  find_unwatched_get_clause_neq_L:
-    \<open>get_clauses_wl S ! watched_by_app S L C ! xj \<noteq> L\<close> (is ?neq)
-  if
-    find_unw: \<open>unit_prop_body_wl_D_find_unwatched_inv (Some xj) (watched_by S L ! C) S\<close> and
-    inv: \<open>unit_prop_body_wl_D_inv S C L\<close>
-  for S C xj L
-proof (rule ccontr)
-  have is_\<L>\<^sub>a\<^sub>l\<^sub>l_alt_def_sym: \<open>is_\<L>\<^sub>a\<^sub>l\<^sub>l (all_lits_of_mm A) \<longleftrightarrow> atms_of \<L>\<^sub>a\<^sub>l\<^sub>l = atms_of_mm A\<close> for A
-    unfolding is_\<L>\<^sub>a\<^sub>l\<^sub>l_alt_def by metis
-  assume eq[simplified, simp]: \<open>\<not> ?neq\<close>
-  let ?C = \<open>get_clauses_wl S ! watched_by_app S L C\<close>
-  let ?L = \<open>get_clauses_wl S ! watched_by_app S L C ! xj\<close>
-  have corr: \<open>correct_watching S\<close> and
-    alien: \<open>cdcl\<^sub>W_restart_mset.no_strange_atm
-      (state\<^sub>W_of (twl_st_of (Some L) (st_l_of_wl (Some (L, C)) S)))\<close> and
-    dist: \<open>cdcl\<^sub>W_restart_mset.distinct_cdcl\<^sub>W_state
-       (state\<^sub>W_of (twl_st_of (Some L) (st_l_of_wl (Some (L, C)) S)))\<close>
-    using inv unfolding unit_prop_body_wl_D_inv_def unit_prop_body_wl_inv_def
-    unfolding correct_watching.simps twl_struct_invs_def cdcl\<^sub>W_restart_mset.cdcl\<^sub>W_all_struct_inv_def
-      by fast+
-  moreover have \<open>watched_by_app S L C < length (get_clauses_wl S)\<close>
-    using inv by (blast intro: unit_prop_body_wl_D_invD)
-  moreover have \<open>watched_by_app S L C > 0\<close>
-    using inv by (blast intro: unit_prop_body_wl_D_invD)
-  ultimately have in_watched: \<open>watched_by_app S L C \<in># mset (watched_by S L)\<close>
-    using inv by (auto simp: watched_by_app_def dest: unit_prop_body_wl_D_invD)
-
-  have \<open>literals_are_\<L>\<^sub>i\<^sub>n S\<close>
-    using inv by (blast intro: unit_prop_body_wl_D_invD)
-  moreover have \<open>L \<in> snd ` D\<^sub>0\<close>
-    using inv by (auto intro: unit_prop_body_wl_D_invD)
-  ultimately have
-    \<open>L \<in># all_lits_of_mm (mset `# mset (tl (get_clauses_wl S)) + get_unit_init_clss S)\<close>
-    using alien
-    by (cases S)
-        (auto 5 5 simp: get_unit_init_clss_def clauses_def mset_take_mset_drop_mset drop_Suc
-        mset_take_mset_drop_mset' cdcl\<^sub>W_restart_mset.no_strange_atm_def
-        is_\<L>\<^sub>a\<^sub>l\<^sub>l_alt_def_sym in_all_lits_of_mm_ain_atms_of_iff in_\<L>\<^sub>a\<^sub>l\<^sub>l_atm_of_in_atms_of_iff
-        dest: in_atms_of_mset_takeD)
-    then have H: \<open>mset (watched_by S L) =
-      mset_set {x. Suc 0 \<le> x \<and> x < length (get_clauses_wl S) \<and>
-         L \<in> set (watched_l (get_clauses_wl S ! x))}\<close>
-      using corr by (cases S)
-          (auto simp: correct_watching.simps watched_by_app_def clause_to_update_def
-          get_unit_init_clss_def)
-  have L_in_watched: \<open>L \<in> set (watched_l ?C)\<close>
-    using in_watched unfolding H
-    by (cases S)
-        (auto simp: correct_watching.simps watched_by_app_def clause_to_update_def
-        get_unit_init_clss_def)
-  have \<open>xj \<ge> 2\<close> and \<open>xj < length (get_clauses_wl S ! watched_by_app S L C)\<close>
-    using find_unw unfolding unit_prop_body_wl_D_find_unwatched_inv_def
-      unit_prop_body_wl_find_unwatched_inv_def
-    by (cases S; auto simp: watched_by_app_def)+
-
-  then have L_in_unwatched: \<open>L \<in> set (unwatched_l ?C)\<close>
-    by (auto simp: in_set_drop_conv_nth intro!: exI[of _ xj])
-  have \<open>distinct_mset_set (mset ` set (tl (get_clauses_wl S)))\<close>
-    apply (subst append_take_drop_id[of \<open>get_learned_wl S\<close>, symmetric])
-    using dist unfolding cdcl\<^sub>W_restart_mset.distinct_cdcl\<^sub>W_state_def set_append
-    by (cases S)
-        (auto simp: mset_take_mset_drop_mset image_Un drop_Suc)
-  then have dist_C: \<open>distinct ?C\<close>
-    using inv by (auto simp: mset_take_mset_drop_mset intro: unit_prop_body_wl_D_invD)
-  then show False
-    using L_in_watched L_in_unwatched by (cases ?C; cases \<open>tl ?C\<close>; cases \<open>tl (tl ?C)\<close>) auto
-qed
-
+(* TODO Kill *)
 lemma update_clause_wl_code_update_clause_wl[sepref_fr_rules]:
   \<open>(uncurry5 update_clause_wl_code, uncurry5 update_clause_wl) \<in>
     [\<lambda>(((((L, C), w), i), f), S).
@@ -810,6 +342,7 @@ proof -
     hr_comp (nat_assn *a twl_st_heur_assn) (nat_rel \<times>\<^sub>f twl_st_heur)\<close>
     (is \<open>_ \<in> [?pre']\<^sub>a ?im' \<rightarrow> ?f'\<close>)
     using hfref_compI_PRE_aux[OF update_clause_wl_code update_clause_wl_heur_update_clause_wl]
+    unfolding update_clause_wl_code_pre_def
     .
   have [dest]: \<open>literals_are_in_\<L>\<^sub>i\<^sub>n_mm (mset `# mset (tl (get_clauses_wl S)))\<close>
     if \<open>unit_prop_body_wl_D_inv S w L\<close>
@@ -867,32 +400,15 @@ proof -
 qed
 
 
-definition propagate_lit_wl_heur
-  :: \<open>nat literal \<Rightarrow> nat \<Rightarrow> nat \<Rightarrow> twl_st_wl_heur \<Rightarrow> twl_st_wl_heur\<close>
-where
-  \<open>propagate_lit_wl_heur = (\<lambda>L' C i (M, N, U, D, Q, W, vm, \<phi>, clvls, cach, lbd, stats).
-      let N' = list_update N C (swap (N!C) 0 (fast_minus 1 i)) in
-      (Propagated L' C # M, N', U, D, add_mset (-L') Q, W, vm, \<phi>, clvls, cach, lbd,
-         incr_propagation stats))\<close>
-
-lemma propagate_lit_wl_heur_propagate_lit_wl:
-  \<open>(uncurry3 (RETURN oooo propagate_lit_wl_heur), uncurry3 (RETURN oooo propagate_lit_wl)) \<in>
-  [\<lambda>(((L, C), i), S). undefined_lit (get_trail_wl S) L \<and> get_conflict_wl S = None]\<^sub>f
-  Id \<times>\<^sub>f nat_rel \<times>\<^sub>f nat_rel \<times>\<^sub>f twl_st_heur \<rightarrow> \<langle>twl_st_heur\<rangle>nres_rel\<close>
-  by (intro frefI nres_relI)
-    (auto simp: twl_st_heur_def propagate_lit_wl_heur_def propagate_lit_wl_def
-      vmtf_consD)
-
 sepref_thm propagate_lit_wl_code
   is \<open>uncurry3 (RETURN oooo (PR_CONST propagate_lit_wl_heur))\<close>
-  :: \<open>[\<lambda>(((L, C), i), S). undefined_lit (get_trail_wl_heur S) L \<and> L \<in> snd ` D\<^sub>0 \<and>
-       1 - i < length (get_clauses_wl_heur S ! C) \<and> i \<le> 1 \<and>
-       C < length (get_clauses_wl_heur S)]\<^sub>a
+  :: \<open>[propagate_lit_wl_heur_pre]\<^sub>a
       unat_lit_assn\<^sup>k *\<^sub>a nat_assn\<^sup>k *\<^sub>a nat_assn\<^sup>k *\<^sub>a twl_st_heur_assn\<^sup>d \<rightarrow> twl_st_heur_assn\<close>
   unfolding PR_CONST_def propagate_lit_wl_heur_def twl_st_heur_assn_def
     cons_trail_Propagated_def[symmetric]
   supply [[goals_limit=1]]length_rll_def[simp] length_ll_def[simp]
   unfolding update_clause_wl_heur_def twl_st_heur_assn_def Array_List_Array.swap_ll_def[symmetric]
+    propagate_lit_wl_heur_pre_def
   by sepref
 
 
@@ -903,7 +419,7 @@ concrete_definition (in -) propagate_lit_wl_code
 prepare_code_thms (in -) propagate_lit_wl_code_def
 
 lemmas propagate_lit_wl_code[sepref_fr_rules] =
-  propagate_lit_wl_code.refine[OF isasat_input_bounded_nempty_axioms]
+  propagate_lit_wl_code.refine[OF isasat_input_bounded_nempty_axioms, unfolded PR_CONST_def]
 
 lemma propagate_lit_wl_code_propagate_lit_wl[sepref_fr_rules]:
   \<open>(uncurry3 propagate_lit_wl_code, uncurry3 (RETURN oooo propagate_lit_wl)) \<in>
@@ -925,6 +441,7 @@ proof -
     (is \<open>_ \<in> [?pre']\<^sub>a ?im' \<rightarrow> ?f'\<close>)
     using hfref_compI_PRE_aux[OF propagate_lit_wl_code[unfolded PR_CONST_def]
        propagate_lit_wl_heur_propagate_lit_wl]
+    unfolding propagate_lit_wl_heur_pre_def
     .
   have pre: \<open>?pre' x\<close> if \<open>?pre x\<close> for x
     using that unfolding comp_PRE_def twl_st_heur_def
@@ -940,50 +457,6 @@ proof -
      defer
     using H unfolding im f PR_CONST_def apply assumption
     using pre ..
-qed
-
-lemma undefined_lit_polarity_st_iff:
-   \<open>undefined_lit (get_trail_wl S) L \<longleftrightarrow>
-      polarity_st S L \<noteq> Some True \<and> polarity_st S L \<noteq> Some False\<close>
-  by (auto simp: polarity_st_def polarity_def)
-
-lemma find_unwatched_le_length:
-  \<open>xj < length (get_clauses_wl S ! watched_by_app S L C)\<close>
-  if
-    find_unw: \<open>RETURN (Some xj) \<le> find_unwatched_wl_st S (watched_by_app S L C)\<close>
-  for S L C xj
-  using that unfolding find_unwatched_wl_st_def find_unwatched_l_def
-  by (cases S) auto
-
-lemma find_unwatched_in_D\<^sub>0: \<open>get_clauses_wl S ! watched_by_app S L C ! xj \<in> snd ` D\<^sub>0\<close>
-  if
-    find_unw: \<open>RETURN (Some xj) \<le> find_unwatched_wl_st S (watched_by_app S L C)\<close> and
-    inv: \<open>unit_prop_body_wl_D_inv S C L\<close>
-  for S C xj L
-proof -
-  have \<open>literals_are_\<L>\<^sub>i\<^sub>n S\<close>
-    using inv by (blast intro: unit_prop_body_wl_D_invD)
-  moreover {
-    have xj: \<open>xj < length (get_clauses_wl S ! watched_by_app S L C)\<close>
-      using find_unw by (cases S) (auto simp: find_unwatched_wl_st_def find_unwatched_l_def)
-    have \<open>watched_by_app S L C < length (get_clauses_wl S)\<close> \<open>watched_by_app S L C > 0\<close>
-      using inv by (blast intro: unit_prop_body_wl_D_invD)+
-    then have \<open>get_clauses_wl S ! watched_by_app S L C ! xj \<in>#
-      all_lits_of_mm (mset `# mset (tl (get_clauses_wl S)))\<close>
-      using xj
-      by (cases S)
-          (auto simp: clauses_def watched_by_app_def mset_take_mset_drop_mset
-          in_all_lits_of_mm_ain_atms_of_iff atms_of_ms_def nth_in_set_tl
-          intro!: bexI[of _ \<open>get_clauses_wl S ! watched_by_app S L C\<close>])
-    then have \<open>get_clauses_wl S ! watched_by_app S L C ! xj \<in>#
-      all_lits_of_mm (cdcl\<^sub>W_restart_mset.clauses (state\<^sub>W_of (twl_st_of None (st_l_of_wl None S))))\<close>
-      apply (subst (asm)(3) append_take_drop_id[of \<open>get_learned_wl S\<close>, symmetric])
-      unfolding mset_append
-      by (cases S)
-          (auto simp: clauses_def watched_by_app_def mset_take_mset_drop_mset'
-          all_lits_of_mm_union drop_Suc) }
-  ultimately show ?thesis
-    by (auto simp: image_image is_\<L>\<^sub>a\<^sub>l\<^sub>l_def)
 qed
 
 end
@@ -1003,7 +476,6 @@ lemma unit_propagation_inner_loop_body_wl_D_helper:
   by (rule literals_are_\<L>\<^sub>i\<^sub>n_literals_are_in_\<L>\<^sub>i\<^sub>n_trail[of _ \<open>Some (a, ba)\<close>])
     auto
 
-
 sepref_thm unit_propagation_inner_loop_body_wl_D
   is \<open>uncurry2 ((PR_CONST unit_propagation_inner_loop_body_wl_D) :: nat literal \<Rightarrow> nat \<Rightarrow>
            nat twl_st_wl \<Rightarrow> (nat \<times> nat twl_st_wl) nres)\<close>
@@ -1022,6 +494,29 @@ sepref_thm unit_propagation_inner_loop_body_wl_D
   unfolding lms_fold_custom_empty swap_ll_def[symmetric]
   unfolding delete_index_and_swap_update_def[symmetric] append_update_def[symmetric]
     find_unwatched_wl_st_heur_def[symmetric] polarity_st_def[symmetric]
+    set_conflict_wl'_alt_def[symmetric] fast_minus_def[symmetric]
+    SET_FALSE_def[symmetric] SET_TRUE_def[symmetric]
+  supply [[goals_limit=1]]
+  by sepref
+
+
+sepref_register find_unwatched_wl_st_heur
+sepref_thm unit_propagation_inner_loop_body_wl_heur
+  is \<open>uncurry2 (PR_CONST unit_propagation_inner_loop_body_wl_heur)\<close>
+  :: \<open>unat_lit_assn\<^sup>k *\<^sub>a nat_assn\<^sup>k *\<^sub>a twl_st_heur_assn\<^sup>d \<rightarrow>\<^sub>a nat_assn *a twl_st_heur_assn\<close>
+  supply
+    if_splits[split] unit_prop_body_wl_D_invD[intro,dest]
+    watched_by_app_def[symmetric,simp]
+    access_lit_in_clauses_def[simp] unit_prop_body_wl_D_invD'[intro]
+    length_rll_def[simp] find_unwatched_not_tauto[dest]
+    unit_propagation_inner_loop_body_wl_D_helper[intro]
+    watched_by_app_heur_code_refine[sepref_fr_rules]
+  supply undefined_lit_polarity_st_iff[iff]
+    unit_prop_body_wl_D_find_unwatched_heur_inv_def[simp]
+  unfolding unit_propagation_inner_loop_body_wl_heur_def length_rll_def[symmetric] PR_CONST_def
+  unfolding nth_rll_def[symmetric]
+  unfolding lms_fold_custom_empty swap_ll_def[symmetric]
+  unfolding delete_index_and_swap_update_def[symmetric] append_update_def[symmetric]
     set_conflict_wl'_alt_def[symmetric] fast_minus_def[symmetric]
     SET_FALSE_def[symmetric] SET_TRUE_def[symmetric]
   supply [[goals_limit=1]]
